fix: update to jump context

lean-formalisation/LeanFormalisation/LBase.lean
@@ -72,7 +72,7 @@ inductive Lang : Tag → Type
 | UnOp (arg : Lang .Expr) (op : UnOp) : Lang .Expr
 | If (cond : Lang .Expr) (e₁ : Lang .Expr) (e₂ : Lang .Expr) : Lang .Expr
 | While (cond : Lang .Expr) (body : Lang .Expr) : Lang .Expr
-| Break : Lang .Expr
+| Break (l : Nat) : Lang .Expr
 | Scope (s : Lang .Stmt) (res : Lang .Expr) : Lang .Expr
 -- # Stmt
 | Decl (type : Ty) (e : Lang .Expr) : Lang .Stmt
@@ -83,6 +83,7 @@ inductive Lang : Tag → Type
 notation:100 s₁:100 ";" s₂:101 => Lang.Seq s₁ s₂
 notation x "::=" exp => Lang.Assign x exp
 abbrev Ctx := List Ty
+abbrev JCtx := Nat
 notation Γ₁ "("x")" "=" type => x < List.length Γ₁ ∧ Γ₁[x]? = Option.some type
 
 def langShift {tg : Tag} (l : Nat) : Lang tg → Lang tg
@@ -105,8 +106,8 @@ def langShift {tg : Tag} (l : Nat) : Lang tg → Lang tg
   .If (langShift l cond) (langShift l e₁) (langShift l e₂)
 | .While (cond : Lang .Expr) (body : Lang .Expr) =>
   .While (langShift l cond) (langShift l body)
-| .Break =>
-  .Break
+| .Break l =>
+  .Break l
 | .Scope (s : Lang .Stmt) (res : Lang .Expr) =>
   .Scope (langShift l s) (langShift l res)
 -- # Stmt
@@ -122,75 +123,75 @@ def langShift {tg : Tag} (l : Nat) : Lang tg → Lang tg
 section Types
 
 inductive TypR : Tag → Type
-| Stmt (Γ₁ : Ctx) : TypR .Stmt
+| Stmt (Γ₁ : Ctx) (Δ₁ : JCtx) : TypR .Stmt
 | Expr (type : Ty) : TypR .Expr
 
-inductive Typ : (tg : Tag) → Ctx → Lang tg → TypR tg → Prop
+inductive Typ : (tg : Tag) → Ctx → JCtx → Lang tg → TypR tg → Prop
 -- # Expr
 | TrueConst :
-  Typ .Expr Γ₁ .True (.Expr .bool)
+  Typ .Expr Γ₁ Δ₁ .True (.Expr .bool)
 | FalseConst :
-  Typ .Expr Γ₁ .False (.Expr .bool)
+  Typ .Expr Γ₁ Δ₁ .False (.Expr .bool)
 | NatConst (n : Nat) :
-  Typ .Expr Γ₁ (.Nat n) (.Expr .nat)
+  Typ .Expr Γ₁ Δ₁ (.Nat n) (.Expr .nat)
 | UnitConst :
-  Typ .Expr Γ₁ .Unit (.Expr .unit)
+  Typ .Expr Γ₁ Δ₁ .Unit (.Expr .unit)
 | VarAccess (x : VarName) (type : Ty) :
   (Γ₁(x) = type) →
-  Typ .Expr Γ₁ (.Var x) (.Expr type)
+  Typ .Expr Γ₁ Δ₁ (.Var x) (.Expr type)
 | UnOp (arg : Lang .Expr) (op : UnOp) :
-  Typ .Expr Γ₁ arg (.Expr op.args.1) →
-  Typ .Expr Γ₁ (.UnOp arg op) (.Expr op.args.2)
+  Typ .Expr Γ₁ Δ₁ arg (.Expr op.args.1) →
+  Typ .Expr Γ₁ Δ₁ (.UnOp arg op) (.Expr op.args.2)
 | BinOp (arg₁ arg₂ : Lang .Expr) (op : BinOp) :
-  Typ .Expr Γ₁ arg₁ (.Expr op.args.1) →
-  Typ .Expr Γ₁ arg₂ (.Expr op.args.2) →
-  Typ .Expr Γ₁ (.BinOp arg₁ arg₂ op) (.Expr op.args.3)
+  Typ .Expr Γ₁ Δ₁ arg₁ (.Expr op.args.1) →
+  Typ .Expr Γ₁ Δ₁ arg₂ (.Expr op.args.2) →
+  Typ .Expr Γ₁ Δ₁ (.BinOp arg₁ arg₂ op) (.Expr op.args.3)
 | IfExpr (cond : Lang .Expr) (e₁ : Lang .Expr) (e₂ : Lang .Expr) (type : Ty) :
-  Typ .Expr Γ₁ cond (.Expr .bool) →
-  Typ .Expr Γ₁ e₁ (.Expr type) →
-  Typ .Expr Γ₁ e₂ (.Expr type) →
-  Typ .Expr Γ₁ (.If cond e₁ e₂) (.Expr type)
+  Typ .Expr Γ₁ Δ₁ cond (.Expr .bool) →
+  Typ .Expr Γ₁ Δ₁ e₁ (.Expr type) →
+  Typ .Expr Γ₁ Δ₁ e₂ (.Expr type) →
+  Typ .Expr Γ₁ Δ₁ (.If cond e₁ e₂) (.Expr type)
 | WhileExpr (cond : Lang .Expr) (body : Lang .Expr) :
-  Typ .Expr Γ₁ cond (.Expr .bool) →
-  Typ .Expr Γ₁ body (.Expr .unit) →
-  Typ .Expr Γ₁ (.While cond body) (.Expr .unit)
-| BreakExpr (type : Ty) :
-  Typ .Expr Γ₁ .Break (.Expr .unit)
+  Typ .Expr Γ₁ Δ₁ cond (.Expr .bool) →
+  Typ .Expr Γ₁ (Δ₁ + 1) body (.Expr .unit) →
+  Typ .Expr Γ₁ Δ₁ (.While cond body) (.Expr .unit)
+| BreakExpr (type : Ty) (l : Nat) :
+  l < Δ₁ →
+  Typ .Expr Γ₁ Δ₁ (.Break l) (.Expr .unit)
 | ScopeExpr (s : Lang .Stmt) (e : Lang .Expr) (type : Ty) :
-  Typ .Stmt Γ₁ s (.Stmt Γ₂) →
-  Typ .Expr Γ₂ e (.Expr type) →
-  Typ .Expr Γ₁ (.Scope s e) (.Expr type)
+  Typ .Stmt Γ₁ Δ₁ s (.Stmt Γ₂ Δ₁) →
+  Typ .Expr Γ₂ Δ₁ e (.Expr type) →
+  Typ .Expr Γ₁ Δ₁ (.Scope s e) (.Expr type)
 -- # Stmt
 | VarDecl (e : Lang .Expr) (type : Ty) :
-  Typ .Expr Γ₁ e (.Expr type) →
-  Typ .Stmt Γ₁ (.Decl type e) (.Stmt (type :: Γ₁))
+  Typ .Expr Γ₁ Δ₁ e (.Expr type) →
+  Typ .Stmt Γ₁ Δ₁ (.Decl type e) (.Stmt (type :: Γ₁) Δ₁)
 | VarAssign (x : VarName) (e : Lang .Expr) (type : Ty) :
-  Typ .Expr Γ₁ e (.Expr type) → (Γ₁(x) = type) →
-  Typ .Stmt Γ₁ (.Assign x e) (.Stmt Γ₁)
+  Typ .Expr Γ₁ Δ₁ e (.Expr type) → (Γ₁(x) = type) →
+  Typ .Stmt Γ₁ Δ₁ (.Assign x e) (.Stmt Γ₁ Δ₁)
 | Seq (s₁ s₂ : Lang .Stmt) :
-  Typ .Stmt Γ₁ s₁ (.Stmt Γ₂) →
-  Typ .Stmt Γ₂ s₂ Γ₃ →
-  Typ .Stmt Γ₁ (s₁; s₂) Γ₃
+  Typ .Stmt Γ₁ Δ₁ s₁ (.Stmt Γ₂ Δ₂) →
+  Typ .Stmt Γ₂ Δ₂ s₂ Γ₃ →
+  Typ .Stmt Γ₁ Δ₁ (s₁; s₂) Γ₃
 | Do (e : Lang .Expr) (type : Ty) :
-  Typ .Expr Γ₁ e (.Expr type) →
-  Typ .Stmt Γ₁ (.Do e) (.Stmt Γ₁)
+  Typ .Expr Γ₁ Δ₁ e (.Expr type) →
+  Typ .Stmt Γ₁ Δ₁ (.Do e) (.Stmt Γ₁ Δ₁)
 
 end Types
 
 section TypeProperties
 
 theorem lang_det (Γ₁ : Ctx) (tg : Tag) (Γ₂ Γ₃ : TypR tg) (s : Lang tg) :
-  Typ tg Γ₁ s Γ₂ → Typ tg Γ₁ s Γ₃ → Γ₂ = Γ₃ := by
+  Typ tg Γ₁ Δ₁ s Γ₂ → Typ tg Γ₁ Δ₁ s Γ₃ → Γ₂ = Γ₃ := by
     intro h1 h2
     unhygienic induction h1 <;> try grind
     all_goals
     { cases h2
       grind }
 
-
 theorem typ_permutation (Γ₁ Γ₂ : Ctx) (tg : Tag) (Γ₃ : TypR tg) (e : Lang tg) :
   (∀ tp x, (Γ₁(x) = tp) ↔ Γ₂(x) = tp) →
-  Typ tg Γ₁ e Γ₃ → Typ tg Γ₂ e Γ₃ := by
+  Typ tg Γ₁ Δ₁ e Γ₃ → Typ tg Γ₂ Δ₁ e Γ₃ := by
     intro hg
     have leq : Γ₁.length = Γ₂.length := by
       by_cases h1: Γ₂.length < Γ₁.length
@@ -216,14 +217,14 @@ theorem typ_permutation (Γ₁ Γ₂ : Ctx) (tg : Tag) (Γ₃ : TypR tg) (e : La
 
 def TypR.extL (Γ₁ : Ctx) (tg : Tag) : TypR tg → TypR tg
 | .Expr type => .Expr type
-| .Stmt Γ₂ => .Stmt (Γ₁ ++ Γ₂)
+| .Stmt Γ₂ Δ₂ => .Stmt (Γ₁ ++ Γ₂) Δ₂
 
 def TypR.extR (Γ₁ : Ctx) (tg : Tag) : TypR tg → TypR tg
 | .Expr type => .Expr type
-| .Stmt Γ₂ => .Stmt (Γ₂ ++ Γ₁)
+| .Stmt Γ₂ Δ₂ => .Stmt (Γ₂ ++ Γ₁) Δ₂
 
 lemma stmt_mono (Γ₁ : Ctx) (tg : Tag) (Γ₂ : TypR tg) (s : Lang tg) :
-  Typ tg Γ₁ s Γ₂ → ∃ Γ₃ : TypR tg, Γ₃.extR Γ₁ = Γ₂ := by
+  Typ tg Γ₁ Δ₁ s Γ₂ → ∃ Γ₃ : TypR tg, Γ₃.extR Γ₁ = Γ₂ := by
     intro hs
     unhygienic induction hs <;> try grind
     all_goals try
@@ -231,26 +232,32 @@ lemma stmt_mono (Γ₁ : Ctx) (tg : Tag) (Γ₂ : TypR tg) (s : Lang tg) :
       rw [TypR.extR] }
     { eapply Exists.intro
       rw [TypR.extR]
-      have : ?VarDecl.h.Γ₂ = [type] := by rfl
+      rotate_left
+      { exact [type] }
+      { exact Δ₁_1 }
       grind }
     { eapply Exists.intro
       rw [TypR.extR]
-      have : ?VarAssign.h.Γ₂ = [] := by rfl
+      rotate_left
+      { exact [] }
+      { exact Δ₁_1 }
       grind }
     { have ⟨g, hg⟩:= a_ih
       unhygienic cases g
       have ⟨g1, hg1⟩:= a_ih_1
       unhygienic cases g1
       simp only [TypR.extR] at *
-      exists TypR.Stmt (Γ₁_3 ++ Γ₁_2)
+      exists TypR.Stmt (Γ₁_3 ++ Γ₁_2) Δ₁_3
       grind }
     eapply Exists.intro
     rw [TypR.extR]
-    have : ?Do.h.Γ₂ = [] := by rfl
+    rotate_left
+    { exact [] }
+    { exact Δ₁_1 }
     grind
 
 
-lemma stmt_decl (type : Ty) : Typ .Stmt Γ₁ (.Decl type e) (.Stmt Γ₂) → Γ₂ = type :: Γ₁ := by
+lemma stmt_decl (type : Ty) : Typ .Stmt Γ₁ Δ₁ (.Decl type e) (.Stmt Γ₂ Δ₁) → Γ₂ = type :: Γ₁ := by
   intro h
   cases h
   rfl
@@ -265,7 +272,7 @@ lemma p_index_r (Γ₁ Γ₂ : Ctx) (i : Nat) :
 
 
 theorem lang_extension (tg : Tag) (e : Lang tg) (res : TypR tg) (Γ₁ Γ₂ : Ctx) :
-  Typ tg Γ₁ e res → Typ tg (Γ₁ ++ Γ₂) (e) (res.extR Γ₂) := by
+  Typ tg Γ₁ Δ₁ e res → Typ tg (Γ₁ ++ Γ₂) Δ₁ (e) (res.extR Γ₂) := by
     intro h
     unhygienic induction h generalizing Γ₂ <;>try solve_by_elim
     { rw [TypR.extR]
@@ -315,12 +322,16 @@ inductive Cont
 | scopeExitK (n : Nat)
 | exprStmtK
 
+abbrev JStackCtx := List (Nat × List Cont)
 
 structure CEK where
   C : Control
   E : Environment
+  J : JStackCtx
   K : List Cont
 
+-- Do we need this relation in the current Jump Context implementation?
+/-
 inductive PopLoopK : List Cont → List Cont → Nat → Prop
 | loopK (c body : Lang .Expr) (n : Nat) (rest : List Cont) :
   PopLoopK (.loopK c body n :: rest) rest n
@@ -329,175 +340,176 @@ inductive PopLoopK : List Cont → List Cont → Nat → Prop
 | skip (k : Cont) (rest result : List Cont) (n : Nat) :
   PopLoopK rest result n →
   PopLoopK (k :: rest) result n
+-/
 
 inductive Eval : CEK → CEK → Prop
 -- # Expr
 | Val (v : Value) :
   Eval
-    ⟨.sourceExpr (liftValue v), E, K⟩
-    ⟨.value v, E, K⟩
+    ⟨.sourceExpr (liftValue v), E, J, K⟩
+    ⟨.value v, E, J, K⟩
 | Var (v : Value) (x : VarName) :
   Eval
-    ⟨.sourceExpr (.Var x), E, K⟩
-    ⟨.value (E[x]!), E, K⟩
+    ⟨.sourceExpr (.Var x), E, J, K⟩
+    ⟨.value (E[x]!), E, J, K⟩
 | VarDecl (type : Ty) (e : Lang .Expr) :
   Eval
-    ⟨.sourceStmt (.Decl type e), E, K⟩
-    ⟨.sourceExpr e, E, (.declK type) :: K⟩
+    ⟨.sourceStmt (.Decl type e), E, J, K⟩
+    ⟨.sourceExpr e, E, J, (.declK type) :: K⟩
 | Assign (x : VarName) (e : Lang .Expr) :
   Eval
-    ⟨.sourceStmt (.Assign x e), E, K⟩
-    ⟨.sourceExpr e, E, (.assignK x) :: K⟩
+    ⟨.sourceStmt (.Assign x e), E, J, K⟩
+    ⟨.sourceExpr e, E, J, (.assignK x) :: K⟩
 | Seq (s₁ s₂ : Lang .Stmt) :
   Eval
-    ⟨.sourceStmt (.Seq s₁ s₂), E, K⟩
-    ⟨.sourceStmt s₁, E, (.seqK s₂) :: K⟩
+    ⟨.sourceStmt (.Seq s₁ s₂), E, J, K⟩
+    ⟨.sourceStmt s₁, E, J, (.seqK s₂) :: K⟩
 | ExprStmt (e : Lang .Expr) :
   Eval
-    ⟨.sourceStmt (.Do e), E, K⟩
-    ⟨.sourceExpr e, E, .exprStmtK :: K⟩
+    ⟨.sourceStmt (.Do e), E, J, K⟩
+    ⟨.sourceExpr e, E, J, .exprStmtK :: K⟩
 | BinOp (e₁ e₂ : Lang .Expr) (op : BinOp) :
   Eval
-    ⟨.sourceExpr (.BinOp e₁ e₂ op), E, K⟩
-    ⟨.sourceExpr e₁, E, (.binopLK op e₂) :: K⟩
+    ⟨.sourceExpr (.BinOp e₁ e₂ op), E, J, K⟩
+    ⟨.sourceExpr e₁, E, J, (.binopLK op e₂) :: K⟩
 | UnOp (e : Lang .Expr) (op : UnOp) :
   Eval
-    ⟨.sourceExpr (.UnOp e op), E, K⟩
-    ⟨.sourceExpr e, E, (.unopK op) :: K⟩
+    ⟨.sourceExpr (.UnOp e op), E, J, K⟩
+    ⟨.sourceExpr e, E, J, (.unopK op) :: K⟩
 | If (e : Lang .Expr) (s₁ s₂ : Lang .Expr) :
   Eval
-    ⟨.sourceExpr (.If e s₁ s₂), E, K⟩
-    ⟨.sourceExpr e, E, (.ifCondK s₁ s₂) :: K⟩
+    ⟨.sourceExpr (.If e s₁ s₂), E, J, K⟩
+    ⟨.sourceExpr e, E, J, (.ifCondK s₁ s₂) :: K⟩
 | While (c : Lang .Expr) (body : Lang .Expr) :
   Eval
-    ⟨.sourceExpr (.While c body), E, K⟩
-    ⟨.sourceExpr c, E, (.loopK c body E.length) :: K⟩
-| Break (K' : List Cont) (n : Nat) :
-  PopLoopK K K' n →
+    ⟨.sourceExpr (.While c body), E, J, K⟩
+    ⟨.sourceExpr c, E, J, (.loopK c body E.length) :: K⟩
+| Break (K' : List Cont) (l : Nat):
   Eval
-    ⟨.sourceExpr .Break, E, K⟩
-    ⟨.skip, E.drop n, K'⟩
+    ⟨.sourceExpr (.Break l), E, J, K⟩
+    -- was skip before, should it be .skip?
+    ⟨.value .Unit, E.drop (E.length - J[l]!.1), J.drop (l + 1), J[l]!.2⟩
 | Scope (s : Lang .Stmt) (e : Lang .Expr) :
   Eval
-    ⟨.sourceExpr (.Scope s e), E, K⟩
-    ⟨.sourceStmt s, E, .scopeBodyK e E.length :: K⟩
+    ⟨.sourceExpr (.Scope s e), E, J, K⟩
+    ⟨.sourceStmt s, E, J, .scopeBodyK e E.length :: K⟩
 -- # Cont
 | IfTrue (s₁ s₂ : Lang .Expr) :
   Eval
-    ⟨.value .True, E, .ifCondK s₁ s₂ :: K⟩
-    ⟨.sourceExpr e₁, E, K⟩
+    ⟨.value .True, E, J, .ifCondK s₁ s₂ :: K⟩
+    ⟨.sourceExpr s₁, E, J, K⟩
 | IfFalse (s₁ s₂ : Lang .Expr) :
   Eval
-    ⟨.value .False, E, .ifCondK s₁ s₂ :: K⟩
-    ⟨.sourceExpr e₁, E, K⟩
+    ⟨.value .False, E, J, .ifCondK s₁ s₂ :: K⟩
+    ⟨.sourceExpr s₂, E, J, K⟩
 | VarDeclDone (type : Ty) (v : Value) :
   Eval
-    ⟨.value v, E, .declK type :: K⟩
-    ⟨.skip, v :: E, K⟩
+    ⟨.value v, E, J, .declK type :: K⟩
+    ⟨.skip, v :: E, J, K⟩
 | AssignDone (x : VarName) (v : Value) :
   Eval
-    ⟨.value v, E, .assignK x :: K⟩
-    ⟨.skip, E.set x v, K⟩
+    ⟨.value v, E, J, .assignK x :: K⟩
+    ⟨.skip, E.set x v, J, K⟩
 | SeqDone (s₂ : Lang .Stmt) :
   Eval
-    ⟨.skip, E, .seqK s₂ :: K⟩
-    ⟨.sourceStmt s₂, E, K⟩
+    ⟨.skip, E, J, .seqK s₂ :: K⟩
+    ⟨.sourceStmt s₂, E, J, K⟩
 | BinOpL (op : BinOp) (v₁ : Value) (e₂ : Lang .Expr) :
   Eval
-    ⟨.value v₁, E, .binopLK op e₂ :: K⟩
-    ⟨.sourceExpr e₂, E, .binopRK op v₁ :: K⟩
+    ⟨.value v₁, E, J, .binopLK op e₂ :: K⟩
+    ⟨.sourceExpr e₂, E, J, .binopRK op v₁ :: K⟩
 | BinOpR (op : BinOp) (v₁ v₂ result : Value) :
   op.step v₁ v₂ result →
   Eval
-    ⟨.value v₂, E, .binopRK op v₁ :: K⟩
-    ⟨.value result, E, K⟩
+    ⟨.value v₂, E, J, .binopRK op v₁ :: K⟩
+    ⟨.value result, E, J, K⟩
 | UnOpDone (op : UnOp) (v result : Value) :
   op.step v result →
   Eval
-    ⟨.value v, E, .unopK op :: K⟩
-    ⟨.value result, E, K⟩
+    ⟨.value v, E, J, .unopK op :: K⟩
+    ⟨.value result, E, J, K⟩
 | LoopTrue (body : Lang .Expr) (c : Lang .Expr) (n : Nat) :
   Eval
-    ⟨.value .True, E, .loopK c body n :: K⟩
-    ⟨.sourceExpr body, E, .loopK c body n :: K⟩
+    ⟨.value .True, E, J, .loopK c body n :: K⟩
+    ⟨.sourceExpr body, E, ⟨n, K⟩ :: J, .loopContK c body n :: K⟩
 | LoopFalse (body : Lang .Expr) (c : Lang .Expr) (n : Nat) :
   Eval
-    ⟨.value .False, E, .loopK c body n :: K⟩
-    ⟨.value .Unit, E, K⟩
+    ⟨.value .False, E, J, .loopK c body n :: K⟩
+    ⟨.value .Unit, E.drop (E.length - n), J, K⟩
 | LoopCont (body : Lang .Expr) (c : Lang .Expr) (n : Nat) :
   Eval
-    ⟨.value .Unit, E, .loopContK c body n :: K⟩
-    ⟨.sourceExpr c, E, .loopK c body n :: K⟩
+    ⟨.value .Unit, E, ⟨n, K⟩ :: J, .loopContK c body n :: K⟩
+    ⟨.sourceExpr c, E, J, .loopK c body n :: K⟩
 | ScopeBody (body : Lang .Expr) (n : Nat) :
   Eval
-    ⟨.skip, E, .scopeBodyK body n :: K⟩
-    ⟨.sourceExpr body, E, .scopeExitK n :: K⟩
+    ⟨.skip, E, J, .scopeBodyK body n :: K⟩
+    ⟨.sourceExpr body, E, J, .scopeExitK n :: K⟩
 | ScopeExit (body : Lang .Expr) (n : Nat) (v : Value) :
   Eval
-    ⟨.value v, E, .scopeExitK n :: K⟩
-    ⟨.value v, E.drop n, K⟩
+    ⟨.value v, E, J, .scopeExitK n :: K⟩
+    ⟨.value v, E.drop (E.length - n), J, K⟩
 
 
-def initState (s : Lang .Stmt) : CEK := ⟨.sourceStmt s, [], []⟩
+def initState (s : Lang .Stmt) : CEK := ⟨.sourceStmt s, [], [], []⟩
 
-def terminalState (E : Environment) : CEK := ⟨.skip, E, []⟩
+def terminalState (E : Environment) : CEK := ⟨.skip, E, [], []⟩
 
 inductive ContTypeRes : Tag → Type
 | Expr (type : Ty) : ContTypeRes .Expr
 | Stmt : ContTypeRes .Stmt
 
 -- # Expression Continuations
-inductive ContType : (tg : Tag) → Ctx → List Cont → ContTypeRes tg → Prop
+inductive ContType : (tg : Tag) → Ctx → JCtx → List Cont → ContTypeRes tg → Prop
 | IfCondK (s₁ : Lang .Expr) (s₂ : Lang .Expr) (Γ₁ : Ctx) (type : Ty) :
-  Typ .Expr Γ₁ s₁ (.Expr type) →
-  Typ .Expr Γ₁ s₂ (.Expr type) →
-  ContType .Expr Γ₁ K (.Expr type) →
-  ContType .Expr Γ₁ (.ifCondK s₁ s₂ :: K) (.Expr .bool)
+  Typ .Expr Γ₁ Δ₁ s₁ (.Expr type) →
+  Typ .Expr Γ₁ Δ₁ s₂ (.Expr type) →
+  ContType .Expr Γ₁ Δ₁ K (.Expr type) →
+  ContType .Expr Γ₁ Δ₁ (.ifCondK s₁ s₂ :: K) (.Expr .bool)
 | DeclK (type : Ty) (Γ₁ : Ctx) :
-  ContType .Stmt (type :: Γ₁) K .Stmt →
-  ContType .Expr Γ₁ (.declK type :: K) (.Expr type)
+  ContType .Stmt (type :: Γ₁) Δ₁ K .Stmt →
+  ContType .Expr Γ₁ Δ₁ (.declK type :: K) (.Expr type)
 | AssignK (x : VarName) (type : Ty) (Γ₁ : Ctx) :
   (Γ₁[x]! = type) →
-  ContType .Stmt Γ₁ K .Stmt →
-  ContType .Expr Γ₁ (.assignK x :: K) (.Expr type)
+  ContType .Stmt Γ₁ Δ₁ K .Stmt →
+  ContType .Expr Γ₁ Δ₁ (.assignK x :: K) (.Expr type)
 | BinOpLK (Γ₁ : Ctx) (op : BinOp) (e₂ : Lang .Expr) :
-  Typ .Expr Γ₁ e₂ (.Expr op.args.2) →
-  ContType .Expr Γ₁ K (.Expr op.args.out) →
-  ContType .Expr Γ₁ (.binopLK op e₂ :: K) (.Expr op.args.1)
+  Typ .Expr Γ₁ Δ₁ e₂ (.Expr op.args.2) →
+  ContType .Expr Γ₁ Δ₁ K (.Expr op.args.out) →
+  ContType .Expr Γ₁ Δ₁ (.binopLK op e₂ :: K) (.Expr op.args.1)
 | BinOpRK (Γ₁ : Ctx) (op : BinOp) (v₁ : Value) :
   value_type v₁ op.args.1 →
-  ContType .Expr Γ₁ K (.Expr op.args.out) →
-  ContType .Expr Γ₁ (.binopRK op v₁ :: K) (.Expr op.args.2)
+  ContType .Expr Γ₁ Δ₁ K (.Expr op.args.out) →
+  ContType .Expr Γ₁ Δ₁ (.binopRK op v₁ :: K) (.Expr op.args.2)
 | UnOpK (Γ₁ : Ctx) (op : UnOp) :
-  ContType .Expr Γ₁ K (.Expr op.args.out) →
-  ContType .Expr Γ₁ (.unopK op :: K) (.Expr op.args.1)
+  ContType .Expr Γ₁ Δ₁ K (.Expr op.args.out) →
+  ContType .Expr Γ₁ Δ₁ (.unopK op :: K) (.Expr op.args.1)
 | LoopK (Γ₁ : Ctx) (e : Lang .Expr) (c : Lang .Expr) (n : Nat) :
-  Typ .Expr Γ₁ c (.Expr .bool) →
-  Typ .Expr Γ₁ e (.Expr .unit) →
-  ContType .Expr (Γ₁.drop n) K (.Expr .unit) →
-  ContType .Expr Γ₁ (.loopK c e n :: K) (.Expr .bool)
+  Typ .Expr Γ₁ Δ₁ c (.Expr .bool) →
+  Typ .Expr Γ₁ (Δ₁ + 1) e (.Expr .unit) →
+  ContType .Expr (Γ₁.drop (Γ₁.length - n)) Δ₁ K (.Expr .unit) →
+  ContType .Expr Γ₁ Δ₁ (.loopK c e n :: K) (.Expr .bool)
 | LoopContK (Γ₁ : Ctx) (e : Lang .Expr) (c : Lang .Expr) (n : Nat) :
-  Typ .Expr Γ₁ c (.Expr .bool) →
-  Typ .Expr Γ₁ e (.Expr .unit) →
-  ContType .Expr (Γ₁.drop n) K (.Expr .unit) →
-  ContType .Expr Γ₁ (.loopContK c e n :: K) (.Expr .bool)
+  Typ .Expr Γ₁ Δ₁ c (.Expr .bool) →
+  Typ .Expr Γ₁ (Δ₁ + 1) e (.Expr .unit) →
+  ContType .Expr (Γ₁.drop (Γ₁.length - n)) Δ₁ K (.Expr .unit) →
+  ContType .Expr Γ₁ Δ₁ (.loopContK c e n :: K) (.Expr .bool)
 | ScopeExitK (Γ₁ : Ctx) (n : Nat) (type : Ty) :
-  ContType .Expr (Γ₁.drop n) K (.Expr type) →
-  ContType .Expr Γ₁ (.scopeExitK n :: K) (.Expr type)
+  ContType .Expr (Γ₁.drop (Γ₁.length - n)) Δ₁ K (.Expr type) →
+  ContType .Expr Γ₁ Δ₁ (.scopeExitK n :: K) (.Expr type)
 | ExprStmtK (Γ₁ : Ctx) (type : Ty) :
-  ContType .Stmt Γ₁ K .Stmt →
-  ContType .Expr Γ₁ (.exprStmtK :: K) (.Expr type)
+  ContType .Stmt Γ₁ Δ₁ K .Stmt →
+  ContType .Expr Γ₁ Δ₁ (.exprStmtK :: K) (.Expr type)
 -- # Statement Continuations
 | HaltK (Γ₁ : Ctx) :
-  ContType .Stmt Γ₁ [] .Stmt
+  ContType .Stmt Γ₁ Δ₁ [] .Stmt
 | SeqK (Γ₁ : Ctx) (Γ₂ : Ctx) (s : Lang .Stmt) :
-  Typ .Stmt Γ₁ s (.Stmt Γ₂) →
-  ContType .Stmt Γ₂ K .Stmt →
-  ContType .Stmt Γ₁ (.seqK s :: K) .Stmt
+  Typ .Stmt Γ₁ Δ₁ s (.Stmt Γ₂ Δ₁) →
+  ContType .Stmt Γ₂ Δ₁ K .Stmt →
+  ContType .Stmt Γ₁ Δ₁ (.seqK s :: K) .Stmt
 | ScopeBodyK (Γ₁ : Ctx) (e : Lang .Expr) (type : Ty) (n : Nat) :
-  Typ .Expr Γ₁ e (.Expr type) →
-  ContType .Expr (Γ₁.drop n) K (.Expr type) →
-  ContType .Stmt Γ₁ (.scopeBodyK e n :: K) .Stmt
+  Typ .Expr Γ₁ Δ₁ e (.Expr type) →
+  ContType .Expr (Γ₁.drop (Γ₁.length - n)) Δ₁ K (.Expr type) →
+  ContType .Stmt Γ₁ Δ₁ (.scopeBodyK e n :: K) .Stmt
 
 inductive Coh : Environment → Ctx → Prop
 | CohEmp :
@@ -507,26 +519,38 @@ inductive Coh : Environment → Ctx → Prop
   value_type v type →
   Coh (v :: E) (type :: Γ)
 
+inductive JCoh : JStackCtx → Ctx → JCtx → Prop
+| JCohEmp :
+  JCoh [] [] 0
+| JCohLoop (n : Nat) (Γ₁ : Ctx) (Δ₁ : JCtx) :
+  JCoh J (Γ₁.drop (Γ₁.length - n)) Δ₁ →
+  ContType .Expr (Γ₁.drop (Γ₁.length - n)) Δ₁ K (.Expr .unit) →
+  JCoh (⟨n, K⟩ :: J) Γ₁ (Δ₁ + 1)
+
 inductive Wt : CEK → Prop
 | WtExprE (e : Lang .Expr) (type : Ty) :
   Coh E Γ →
-  Typ .Expr Γ e (.Expr type) →
-  ContType .Expr Γ K (.Expr type) →
-  Wt ⟨.sourceExpr e, E, K⟩
+  JCoh J Γ Δ →
+  Typ .Expr Γ Δ e (.Expr type) →
+  ContType .Expr Γ Δ K (.Expr type) →
+  Wt ⟨.sourceExpr e, E, J, K⟩
 | WtExprS (s : Lang .Stmt) :
   Coh E Γ →
-  Typ .Stmt Γ s (.Stmt Γ₁) →
-  ContType .Stmt Γ₁ K .Stmt →
-  Wt ⟨.sourceStmt s, E, K⟩
+  JCoh J Γ Δ →
+  Typ .Stmt Γ Δ s (.Stmt Γ₁ Δ) →
+  ContType .Stmt Γ₁ Δ K .Stmt →
+  Wt ⟨.sourceStmt s, E, J, K⟩
 | WtContV (v : Value) (type : Ty) :
   Coh E Γ →
+  JCoh J Γ Δ →
   value_type v type →
-  ContType .Expr Γ K (.Expr type) →
-  Wt ⟨.value v, E, K⟩
+  ContType .Expr Γ Δ K (.Expr type) →
+  Wt ⟨.value v, E, J, K⟩
 | WtContS :
   Coh E Γ →
-  ContType .Stmt Γ K .Stmt →
-  Wt ⟨.skip, E, K⟩
+  JCoh J Γ Δ →
+  ContType .Stmt Γ Δ K .Stmt →
+  Wt ⟨.skip, E, J, K⟩
 
 -- do casing on Continuation
 theorem progress (s : CEK) :
@@ -534,7 +558,7 @@ theorem progress (s : CEK) :
   (∃ E, terminalState E = s) ∨ ∃ s', Eval s s' := by
     intro hwt
     unhygienic induction s
-    by_cases ht : ∃ E1, terminalState E1 = ⟨C, E, K⟩
+    by_cases ht : ∃ E1, terminalState E1 = ⟨C, E, J, K⟩
     { grind }
     simp [terminalState] at ht
     right
@@ -542,7 +566,7 @@ theorem progress (s : CEK) :
     stop sorry
 
 lemma lift_value_type (v : Value) (type : Ty) :
-  Typ .Expr Γ (liftValue v) (.Expr type) → value_type v type := by
+  Typ .Expr Γ Δ (liftValue v) (.Expr type) → value_type v type := by
     intro ht
     cases v <;> cases ht <;> grind [value_type]
 
@@ -581,62 +605,49 @@ theorem preservation (s s' : CEK) :
     intro hw he
     unhygienic induction he <;> unhygienic cases hw
     all_goals try
-    { unhygienic cases a_1
+    { unhygienic cases a_2
       apply Wt.WtExprE
       { apply a }
-      { apply a_3 }
+      { apply a_1 }
+      { apply a_4 }
       solve_by_elim }
     { apply Wt.WtContV (type := type)
       { apply a }
-      { apply lift_value_type v type a_1 }
-      apply a_2 }
-    { cases a_1
+      { apply a_1 }
+      { apply lift_value_type v type a_2 }
+      apply a_3 }
+    { cases a_2
       apply Wt.WtContV
       { apply a }
+      { apply a_1 }
       { apply coh_get
         { apply a }
         grind [coh_len] }
       grind }
-    { unhygienic cases a_1
+
+    { unhygienic cases a_2
       apply Wt.WtExprE
       { apply a }
-      { apply a_3 }
+      { apply a_1 }
+      { apply a_4 }
       apply ContType.AssignK <;> grind }
-    { unhygienic cases a_1
+    { /-unhygienic cases a_2
       apply Wt.WtExprS
       { apply a }
-      { apply a_3 }
+      { apply a_1 }
+      { apply a_4 }
       apply ContType.SeqK
       { apply a_4 }
-      apply a_2 }
-    { unhygienic cases a_1
-      apply Wt.WtExprE
-      { apply a }
-      { apply a_3 }
-      apply ContType.LoopK
-      { apply a_3 }
-      { apply a_4 }
-      have : (Γ.drop (E.length)) = [] := by
-        rw [coh_len _ _ a]
-        grind
-      rw [this]
+      apply a_2-/
+      --check Seq rule
       sorry }
     { unhygienic cases a_2
-      apply Wt.WtContS
-      { apply coh_mono
-        apply a_1 }
-      sorry }
-    { unhygienic cases a_1
-      apply Wt.WtExprS
+      apply Wt.WtExprE
       { apply a }
-      { apply a_3 }
-      apply ContType.ScopeBodyK
+      { apply a_1 }
       { apply a_4 }
-      have mono := stmt_mono _ _ _ _ a_3
-      rcases mono with ⟨m, hm⟩
-      simp [TypR.extR] at hm
-      cases m
-      simp at hm
-
+      apply ContType.LoopK
+      { apply a_4 }
+      { apply a_5 }
       sorry }
     stop sorry
